src/FcEtt/ett_path.v
@@ -10,6 +10,10 @@ Require Import FcEtt.toplevel.
 Require Import FcEtt.ett_roleing.
 Require Import FcEtt.ext_wf.
 
+Lemma CasePath_lc : forall F a R, CasePath R a F -> lc_tm a.
+Proof. intros. induction H; eauto.
+Qed.
+
 Lemma CasePath_binds_toplevel : forall F a R, CasePath R a F ->
                      (exists A Rs, binds F (Cs A Rs) toplevel) \/
                      (exists p a0 A0 R0 Rs, binds F (Ax p a0 A0 R0 Rs) toplevel
@@ -35,16 +39,6 @@ Proof. intros. destruct R1, R2; auto. right. intro. inversion H.
        right. intro. inversion H.
 Qed.
 
-Lemma tm_dec : forall (a : tm) b, a = b \/ ~(a = b).
-Proof. intros. generalize dependent b. induction a; destruct b;
-        try destruct nu, nu0; try destruct rho, rho0; try destruct phi, phi0;
-       try (right; intro P; inversion P; fail);
-       try (left; eauto 2; fail); try (
-       match goal with
-        [ b0 : tm, IH : forall b, _ |- _ ] => pose (Q := IH b0); inversion Q;
-        [ left; f_equal; eauto | right; intro P; inversion P; contradiction]
-       end; fail). Admitted.
-
 Lemma match_bullet : forall a p b, MatchSubst a p a_Bullet b -> b = a_Bullet.
 Proof. intros. dependent induction H; auto.
        pose (P := IHMatchSubst ltac:(auto)). rewrite P. auto.
@@ -54,7 +48,8 @@ Lemma match_dec : forall a p, lc_tm a -> MatchSubst a p a_Bullet a_Bullet \/ ~(M
 Proof. intros. generalize dependent a.
        induction p; intros; try (right; intro P; inversion P; fail).
         - destruct nu. destruct a; try (right; intro P; inversion P; fail).
-          destruct nu. destruct p2; try (right; intro P; inversion P; fail).
+          destruct nu; try (right; intro P; inversion P; fail).
+          destruct p2; try (right; intro P; inversion P; fail).
           pose (P := role_dec R0 R). inversion P. subst.
           inversion H; subst. pose (Q := IHp1 a1 H2). inversion Q.
           assert (Q' : a_Bullet = (tm_subst_tm_tm a2 x a_Bullet)). {auto. }
@@ -62,7 +57,6 @@ Proof. intros. generalize dependent a.
           rewrite <- Q' in H0. auto. auto.
           right. intro Q1. inversion Q1; subst. rewrite H10 in H11.
           pose (Q2 := H11). apply match_bullet in Q2. subst. contradiction.
-          right; intro P1; inversion P1; contradiction.
           right; intro P1; inversion P1; contradiction.
           destruct rho. right; intro P1; inversion P1.
           destruct p2; try (right; intro P; inversion P; fail).
@@ -82,20 +76,25 @@ Proof. intros. generalize dependent a.
           right; intro P; inversion P; contradiction.
 Qed.
 
-Lemma CasePath_ValuePath : forall R a F, CasePath R a F -> ValuePath R a F.
+Lemma CasePath_ValuePath : forall R a F, CasePath R a F -> ValuePath a F.
 Proof. intros. induction H; eauto.
-       pose (P := match_dec). pose (Q := P (a_Fam F) p ltac:(auto)).
-       inversion Q. eauto. eauto.
 Qed.
 
+Lemma CasePath_Value : forall R a F, CasePath R a F -> Value R a.
+Proof. intros. pose (P := CasePath_binds_toplevel H).
+       inversion P as [[A [Rs Q]] | [p [a0 [A0 [R0 [Rs [Q1 Q2]]]]]]].
+       pose (Q' := H). apply CasePath_ValuePath in Q'. eauto.
+       pose (Q' := H). apply CasePath_ValuePath in Q'.
+       pose (Q3 := match_dec). pose (Q4 := Q3 a p (CasePath_lc H)).
+       inversion Q4; eauto.
+Qed.
 (*
 Lemma subst_Path : forall F a b R x, lc_tm b -> Value R a ->
-                   ValuePath R (tm_subst_tm_tm b x a) F -> ValuePath R a F.
+                   CasePath R (tm_subst_tm_tm b x a) F -> CasePath R a F.
 Proof. intros. induction a; simpl in H1; auto; try (inversion H1; fail).
-        - inversion H0. inversion H2. inversion H3.
-        - destruct nu. inversion H1.
-          inversion H2; subst. inversion H2; subst.
-          econstructor. auto. eapply IHa1; eauto.
+        - inversion H0; subst; inversion H2.
+        - destruct nu. inversion H1. inversion H1; subst.
+          econstructor. admit.
         - inversion H0; subst. inversion H1; subst. inversion H2; subst.
           econstructor. eapply IHa; eauto.
 Qed.
